coq/bv/InvCond.v
@@ -15,21 +15,28 @@ induction x.
 
 (*Addition*)
 (* x + s = t <=> x = t - s *)
-Theorem bvadd : forall (x s t : bitvector), iff ((bv_add x s) = t) (x = (bv_subt t s)).
+Theorem bvadd : forall (x s t : bitvector), 
+  iff 
+    ((bv_add x s) = t) 
+    (x = (bv_subt t s)).
 Proof.
 Admitted.
 
 
 (*Multiplication*)
 (* x.s = t <=> (-s | s) & t = t *)
-Theorem bvmult_eq : forall (x s t : bitvector), iff ((bv_mult x s) = t) ((bv_and (bv_or (bv_not s) s) t) = t).
+Theorem bvmult_eq : forall (x s t : bitvector), 
+  iff 
+    ((bv_mult x s) = t) 
+    ((bv_and (bv_or (bv_not s) s) t) = t).
 Proof.
 Admitted.
 
 (* x.s != t <=> s != 0 or t != 0 *)
-Theorem bvmult_neq : forall (x s t : bitvector), iff 
-  (~((bv_mult x s) = t)) 
-  ((~(s = zeros (size s))) \/ (~(t = zeros (size t)))).
+Theorem bvmult_neq : forall (x s t : bitvector), 
+  iff 
+    (~((bv_mult x s) = t)) 
+    ((~(s = zeros (size s))) \/ (~(t = zeros (size t)))).
 Proof.
 Admitted.
 
@@ -58,71 +65,126 @@ Admitted.
 
 (*And*)
 (* x & s = t <=> t & s = t*)
-Theorem bvand_eq : forall (x s t : bitvector), iff ((bv_and x s) = t) ((bv_and t s) = t).
+Theorem bvand_eq : forall (x s t : bitvector), 
+  iff 
+    ((bv_and x s) = t) 
+    ((bv_and t s) = t).
 Proof.
 Admitted.
 
 (* x & s != t <=> s != 0 or t != 0 *)
-Theorem bvand_neq : forall (x s t : bitvector), iff 
-  (~((bv_and x s) = t)) 
-  ((bv_and t s) = t).
+Theorem bvand_neq : forall (x s t : bitvector), 
+  iff 
+    (~((bv_and x s) = t)) 
+    ((bv_and t s) = t).
 Proof.
 Admitted.
 
 (*Or*)
 (* x | s = t <=> t & s = t *)
-Theorem bvor_eq : forall (x s t  :bitvector), iff ((bv_or x s) = t) ((bv_and t s) = t).
+Theorem bvor_eq : forall (x s t : bitvector), 
+  iff 
+    ((bv_or x s) = t) 
+    ((bv_and t s) = t).
 Proof.
 Admitted.
 
 (* x | s != t <=> s != ~0 or t != ~0 *)
-Theorem bvor_neq : forall (x s t : bitvector), iff 
-  (~((bv_or x s) = t)) 
-  (~(s = (bv_not (zeros (size s)))) \/ (~(t = (bv_not (zeros (size t)))))).
+Theorem bvor_neq : forall (x s t : bitvector), 
+   iff 
+    (~((bv_or x s) = t)) 
+    (~(s = (bv_not (zeros (size s)))) 
+      \/ 
+      (~(t = (bv_not (zeros (size t)))))).
 Proof.
 Admitted.
 
 (*Logical right shift*)
 (* x >> s = t <=> (t << s) >> s = t *)
+Theorem bvshr_eq : forall (x s t : bitvector), 
+  iff 
+    (bv_shr x s = t) 
+    (bv_shr (bv_shl t s) s = t).
+Proof.
+Admitted.
 
-(* x >> s != t <=> t != 0 or s <u size(s)*)
+(* x >> s != t <=> t != 0 or s <u Nat2BV (size(s))*)
+(*Theorem bvshr_neq : forall (x s t : bitvector),
+  iff
+    (~(bv_shr x s = t))
+    (~(t = zeros (size t)) 
+      \/
+      (bv_ult s (NAT2BV size s))).*)
 
 (* s >> x = t <=> [i=0...size(s)]OR(s >> i = t) *)
 
 (* s >> x != t <=> s != 0 or t != 0 *)
-
+Theorem bvshr_neq2 : forall (x s t : bitvector),
+  iff
+    (~(bv_shr s x = t))
+    (~(s = zeros (size s))
+      \/
+     ~(t = zeros (size t))).
+Proof.
+Admitted.
 
 (*Arithmetic right shift*)
 (* x >>a s = t <=> 
-  (s <u size(s) => (t << s) >>a s = t) and (s >=u size(s) => (t = ~0 or t = 0)) *)
+  (s <u size(s) => (t << s) >>a s = t) 
+    and 
+    (s >=u size(s) => (t = ~0 or t = 0)) *)
 
 (* x >>a s != t <=> T *)
+Theorem bvashr_neq : forall (x s t : bitvector),
+  iff 
+    (~(bv_ashr x s = t))
+    True.
+Proof.
+Admitted.
 
 (* s >>a x = t <=> [i=0...size(s)OR(s >>a i = t) *)
 
 (* s >>a x != t <=> 
   (t != 0 or s!= 0) and (t != ~0 or s !- ~0) *)
-
+Theorem bvashr_neq2 : forall (x s t : bitvector), 
+  iff
+    (~(bv_ashr s x = t))
+    ((~(t = zeros (size t)) \/ ~(s = zeros (size s)))
+      /\
+      (~(t = bv_not (zeros (size t))) \/ ~(s = bv_not (zeros (size s))))).
+Proof.
+Admitted.
 
 (*Logical left shift*)
 (* x << s = t <=> (t >> s) << s = t *)
+Theorem bvshl_eq : forall (x s t : bitvector),
+  iff
+    (bv_shl x s = t)
+    (bv_shl (bv_shr t s) s = t).
+Proof.
+Admitted.
 
 (* x << s != t <=> t != 0 or s <u size(s) *)
 
 (* s << x = t <=> [i=0...size(s)]OR(s << i = t)  *)
 
 (* s << x != t <=> s != 0 or or t != 0 *)
-
+Theorem bvshl_neq2 : forall (x s t : bitvector),
+  iff
+    (~(bv_shl s x = t))
+    (~(s = zeros (size s)) \/ ~(t = zeros (size t))).
+Proof.
+Admitted.
 
 (*Concat*)
 (* x o s = t <=> s = t[size(s) - 1, 0] *)
-Theorem bvconcat1_eq : forall (x s t : bitvector), iff ((bv_concat x s) = t) 
+Theorem bvconcat_eq : forall (x s t : bitvector), iff ((bv_concat x s) = t) 
 (s = extract t (N.to_nat(size(s)) - 1) (0)).
 Proof.
 Admitted.
 
 (* x o s != t <=> T *)
-Theorem bvconcat1_neq : forall (x s t : bitvector), iff (~((bv_concat x s) = t)) (True).
+Theorem bvconcat_neq : forall (x s t : bitvector), iff (~((bv_concat x s) = t)) (True).
 Proof.
 intros x s t.
 split. 
@@ -130,13 +192,13 @@ split.
 - intros H. Admitted.
 
 (* s o x = t <=> s = t[size(t) - 1 : size(t) - size(s)] *)
-Theorem bvconcat2_eq : forall (x s t : bitvector), iff ((bv_concat s x) = t) 
+Theorem bvconcat_eq2 : forall (x s t : bitvector), iff ((bv_concat s x) = t) 
 (s = extract t (N.to_nat(size(t)) - 1) 
                (N.to_nat(size(t)) - N.to_nat(size(s)))).
 Proof. 
 Admitted.
 
-Theorem bvconcat2_neq : forall (x s t : bitvector), iff (~((bv_concat s x) = t)) (True).
+Theorem bvconcat_neq2 : forall (x s t : bitvector), iff (~((bv_concat s x) = t)) (True).
 Proof.
 intros x s t.
 split.
